Added test thm with proof.

basis/HashtableProofScript.sml
@@ -1,6 +1,7 @@
 (*
   Proofs about the Array module.
 *)
+
 open preamble ml_translatorTheory ml_translatorLib cfLib
      mlbasicsProgTheory HashtableProgTheory
 
@@ -9,19 +10,57 @@ val _ = new_theory"HashtableProof";
 val _ = translation_extends "HashtableProg";
 
 val hashtable_st = get_ml_prog_state();
+
 (*  ----------------------------------- *)
 
-(* Theorem hashtable_empty
-  `!v.`
+(* the union of each bucket is the heap *)
+(* the vlv list contains the buckets *)
+(* each bucket only contains keys that hash there *)
 
-Theorem array_alloc_empty_spec
-  `!v.
-     UNIT_TYPE () v ⇒
-     app (p:'ffi ffi_proj) ^(fetch_v "Hashtable.hashtableEmpty" array_st) [v]
-       emp (POSTv av. ARRAY av [])`
-  (prove_array_spec "Array.arrayEmpty"); *)
+val list_union_def = Define `
+  list_union [x] = x /\
+  list_union (x::xs) = mlmap$union x (list_union xs)`
 
+val hashtable_inv_def = Define `
+  hashtable_inv a b hf cmp (h:'a|->'b) vlv =
+    ?buckets.
+      h = to_fmap (list_union buckets) /\
+      LIST_REL (MAP_TYPE a b) buckets vlv /\
+      ARB`;
 
+val REF_NUM_def = Define `
+  REF_NUM loc n =
+    SEP_EXISTS v. REF loc v * & (NUM n v)`;
+
+val REF_ARRAY_def = Define `
+  REF_ARRAY loc content =
+    SEP_EXISTS v. REF loc v * ARRAY v content`;
+
+val HASHTABLE_def = Define
+ `HASHTABLE a b hf cmp (h:'a|->'b) v =
+    SEP_EXISTS ur ar hfv cmpv vlv heuristic_size.
+      &(v = (Conv (SOME (TypeStamp "Hashtable" 8)) [ur; ar; hfv; cmpv]) /\
+        (a --> INT) hf hfv /\
+        (a --> a --> ORDERING_TYPE) cmp cmpv /\
+        hashtable_inv a b hf cmp h vlv) *
+      REF_NUM ur heuristic_size *
+      REF_ARRAY ar vlv`;
+
+Theorem size_test
+  `!a b hf cmp hv.
+    app (p:'ffi ffi_proj) Hashtable_size_v [hv]
+      (HASHTABLE a b hf cmp h hv)
+      (POSTv v. HASHTABLE a b hf cmp h hv)`
+  (xcf_with_def "Hashtable.size" Hashtable_size_v_def
+  \\ simp[REF_NUM_def,HASHTABLE_def]
+  \\ xpull
+  \\ xmatch
+  \\ xapp
+  \\ xsimpl
+  \\ asm_exists_tac
+  \\ simp[]
+  \\ asm_exists_tac
+  \\ xsimpl);
 
 (*  ----------------------------------- *)
 val _ = export_theory();
